proofs/isabelle/SpecRest/core/Semantics.thy
@@ -10,6 +10,8 @@ datatype (plugins only: code size) ir_value =
   | VEntity "String.literal" "String.literal"
   | VSet "ir_value list"
   | VEntityWith "ir_value" "String.literal" "ir_value"
+  | VNone
+  | VSome "ir_value"
 
 type_synonym env = "(String.literal \<times> ir_value) list"
 
@@ -288,6 +290,8 @@ inductive_cases value_has_ty_entity_cases [elim!]:
 inductive_cases value_has_ty_set_cases [elim!]: "value_has_ty \<Gamma> (VSet vs) t"
 inductive_cases value_has_ty_entity_with_cases [elim!]:
   "value_has_ty \<Gamma> (VEntityWith base fld override) t"
+inductive_cases value_has_ty_none_cases [elim!]: "value_has_ty \<Gamma> VNone t"
+inductive_cases value_has_ty_some_cases [elim!]: "value_has_ty \<Gamma> (VSome v) t"
 
 lemma value_has_ty_VBool_iff [simp]:
   "value_has_ty \<Gamma> (VBool b) t \<longleftrightarrow> t = TBool"
@@ -368,6 +372,8 @@ where
 | "check_value_has_ty \<Gamma> (VEntityWith _ _ _) TReal = False"
 | "check_value_has_ty \<Gamma> (VEntityWith _ _ _) (TEnum _) = False"
 | "check_value_has_ty \<Gamma> (VEntityWith _ _ _) (TSet _) = False"
+| "check_value_has_ty \<Gamma> VNone _ = False"
+| "check_value_has_ty \<Gamma> (VSome _) _ = False"
 | "check_value_has_ty_list _ [] _ = True"
 | "check_value_has_ty_list \<Gamma> (v # vs) t =
      (check_value_has_ty \<Gamma> v t \<and> check_value_has_ty_list \<Gamma> vs t)"
@@ -1210,6 +1216,8 @@ where
         Some (VBool True)  \<Rightarrow> eval s st env a
       | Some (VBool False) \<Rightarrow> eval s st env b
       | _ \<Rightarrow> None)"
+| "eval s st env (NoneE _)   = Some VNone"
+| "eval s st env (SomeE e _) = map_option VSome (eval s st env e)"
 
 | "eval_forall_enum s st env var en [] body = Some (VBool True)"
 | "eval_forall_enum s st env var en (mem # rest) body =
