proofs/isabelle/SpecRest/core/Smt.thy
@@ -16,6 +16,8 @@ datatype (plugins only: code size) smt_val =
   | SEntityElem "String.literal" "String.literal"
   | SSet "smt_val list"
   | SEntityWith "smt_val" "String.literal" "smt_val"
+  | SNone
+  | SSome "smt_val"
 
 datatype (plugins only: code size) smt_term =
     BLit bool
@@ -51,6 +53,8 @@ datatype (plugins only: code size) smt_term =
   | TPre "smt_term"
   | TWithRec "smt_term" "String.literal" "smt_term"
   | TIte "smt_term" "smt_term" "smt_term"
+  | TNone
+  | TSome "smt_term"
 
 record smt_model =
   sm_sort_members :: "(String.literal \<times> String.literal list) list"
@@ -315,6 +319,8 @@ where
         Some (SBool True)  \<Rightarrow> smtEval m env a
       | Some (SBool False) \<Rightarrow> smtEval m env b
       | _ \<Rightarrow> None)"
+| "smtEval m env TNone     = Some SNone"
+| "smtEval m env (TSome t) = map_option SSome (smtEval m env t)"
 
 | "smtEval_forall_enum m env var sort_name [] body = Some (SBool True)"
 | "smtEval_forall_enum m env var sort_name (mem # rest) body =
